Basic executable version of semantics without throw, trycatch, guard and call.

Simpl/Semantics.lean
@@ -1,7 +1,6 @@
 import Simpl.Syntax
 import Std
 import Lean
-
 namespace Simpl
 
 abbrev Record := Std.HashMap
@@ -65,21 +64,27 @@ end
 
 -/
 
-mutual
+
+inductive EvalExpr : State → Expression → CVal → Prop
+  | lookup : EvalExpr state (Expression.ident i)  (state.local_variables.findD i 0)
+  | const : EvalExpr _ (Expression.num n) (n.toUInt32)
+  | add : EvalExpr state e₁ v₁ → EvalExpr state e₂ v₂ → EvalExpr state  (Expression.add e₁ e₂) (v₁ + v₂)
+  | sub : EvalExpr state e₁ v₁ → EvalExpr state e₂ v₂ → EvalExpr state  (Expression.sub e₁ e₂) (v₁ - v₂)
+
+-- See: https://leanprover.github.io/lean4/doc/examples/tc.lean.html
 -- eval won't work as function without coinduction
-def SmallStep : State × Statement → State × Statement
-  | (state, Statement.skip) => (state, Statement.skip)
-  | (state, Statement.assign i e) =>
-    let new_local_variables := state.local_variables.insert i (eval_expr state e)
-    ({ state with local_variables := new_local_variables }, Statement.skip)
-  | (state, Statement.seq (Statement.skip) s₂) => step (state,s₂)
-  | (state, Statement.seq s₁ s₂) => match step (state,s₁) with
-    | (state', Statement.skip) => (state',s₂)
-    | (state', s₁') => (state', Statement.seq s₁' s₂)
-  | (state, Statement.conditional e s₁ s₂) =>
-    if eval_expr state e ≠ 0 then step (state, s₁) else step (state, s₂)
-  | (state, w@(Statement.while e s)) =>
-    if eval_expr state e ≠ 0 then (state, Statement.seq s w) else (state, Statement.skip)
+inductive Step : State × Statement → State × Statement → Prop
+  | skip :  Step (state, Statement.skip) (state, Statement.skip)
+  | assign : EvalExpr state e v → Step (state, Statement.assign i e) ({ state with local_variables := state.local_variables.insert i v}, Statement.skip)
+  | seq_skip : Step (state, Statement.seq (Statement.skip) s₂) (state,s₂)
+  | seq_step : Step (state, s₁) (state', s₁') → Step (state, Statement.seq s₁ s₂) (state', Statement.seq s₁' s₂)
+  | conditional_true : EvalExpr state e val → val ≠ 0 → Step (state, Statement.conditional e s₁ s₂) (state, s₁)
+  | conditional_false : EvalExpr state e val → val = 0 → Step (state, Statement.conditional e s₁ s₂) (state, s₁)
+  | while_stop : EvalExpr state e val → val = 0 → Step (state, Statement.while e s) (state, Statement.skip)
+  | while_loop : EvalExpr state e val → val ≠ 0 → Step (state, (Statement.while e s)) (state, Statement.seq s (Statement.while e s))
+-- Removed because of unspported syntax: elaboration function for 'Lean.Parser.Term.namedPattern' has not been implemented w@(Statement.while e s)
+--  | while_loop : EvalExpr state e val → val ≠ 0 → Step (state, w@(Statement.while e s)) (state, Statement.seq s w)
+  /- Ignore throw, trycatch, guard, call for now
   | s@(_, Statement.throw _) => s
   | (state, Statement.trycatch t c) => match step (state,t) with
     | (state', Statement.skip) => (state', Statement.skip)
@@ -87,18 +92,73 @@ def SmallStep : State × Statement → State × Statement
     | (state', t') => (state', t)
   | (state, Statement.guard e₁ e₂ s₁) => (state, Statement.skip) -- TODO: implement
   | (state, Statement.call _) => (state, Statement.skip) -- TODO: implement
+  -/
 
- def eval_expr : State → Expression → CVal
-  | state, Expression.ident i => state.local_variables.findD i 0
-  | _, Expression.num n => n.toUInt32
-  | state, Expression.add e₁ e₂ => eval_expr state e₁ + eval_expr state e₂
-  | state, Expression.sub e₁ e₂ => eval_expr state e₁ - eval_expr state e₂
-end
+-- An issue here is that `Decidable` requires us to give `cval`, whereas we want to compute it.
+def evalExpr (state : State) (e : Expression) : CVal :=
+  match e with
+  | Expression.ident i => state.local_variables.findD i 0
+  | Expression.num n => n.toUInt32
+  | Expression.add e₁ e₂ => evalExpr state e₁ + evalExpr state e₂
+  | Expression.sub e₁ e₂ => evalExpr state e₁ - evalExpr state e₂
+
+-- Similar to idea from Kyle Miller: https://leanprover.zulipchat.com/#narrow/stream/270676-lean4/topic/Hypothesis.20in.20.60match.60/near/328812446
+theorem evalExpr_correct (state : State) (e : Expression) (cval : CVal) : EvalExpr state e cval ↔ (cval = evalExpr state e) :=
+  by
+   constructor
+   -- =>
+   · intro hCval
+     induction hCval <;> simp [evalExpr]
+     -- case mp.sub
+     case mp.sub h₁ h₂ =>
+       rw [h₁, h₂]
+     case mp.add h₁ h₂ =>
+       rw [h₁, h₂]
+   -- <=
+   · intro hEval
+     induction e generalizing cval <;> simp [evalExpr] at hEval <;> simp [hEval]
+      -- case mp.sub
+     case num n =>
+        exact EvalExpr.const
+     case ident i =>
+        exact EvalExpr.lookup
+     case add e₁ e₂ ih_1 ih_2 =>
+        have v₁rfl : evalExpr state e₁ = evalExpr state e₁ := rfl
+        have hv₁ := ih_1 (evalExpr state e₁) v₁rfl
+        have v₂rfl : evalExpr state e₂ = evalExpr state e₂ := rfl
+        have hv₂ := ih_2 (evalExpr state e₂) v₂rfl
+        exact EvalExpr.add hv₁ hv₂
+     case sub e₁ e₂ ih_1 ih_2 =>
+        have v₁rfl : evalExpr state e₁ = evalExpr state e₁ := rfl
+        have hv₁ := ih_1 (evalExpr state e₁) v₁rfl
+        have v₂rfl : evalExpr state e₂ = evalExpr state e₂ := rfl
+        have hv₂ := ih_2 (evalExpr state e₂) v₂rfl
+        exact EvalExpr.sub hv₁ hv₂
+
+instance (state : State) (e : Expression) (cval : CVal) : Decidable (EvalExpr state e cval) :=
+  if h : cval = evalExpr state e
+    then isTrue <| by
+      exact evalExpr_correct state e cval |>.mpr h
+    else isFalse <| by rwa [evalExpr_correct]
+
+def evalStep  : State × Statement → State × Statement
+  | (state, Statement.skip) => (state, Statement.skip)
+  | (state, Statement.assign name expr) =>
+    let state' := {state with local_variables := state.local_variables.insert name (evalExpr state expr)}
+    (state', Statement.skip)
+--  | (state, Statement.seq (Statement.skip) s₂) => (state, s₂)
+  | (state, Statement.seq s₁ s₂) => match evalStep (state, s₁) with
+    | (state', Statement.skip) => (state', s₂)
+    | (state', s₁') => (state', Statement.seq s₁' s₂)
+  | (state, Statement.conditional e s₁ s₂) => if evalExpr state e ≠ 0 then (state, s₁) else (state, s₂)
+  | (state, Statement.while e s) => if (evalExpr state e) ≠ 0 then (state, Statement.seq s (Statement.while e s)) else (state, Statement.skip)
+  -- TODO: throw, trycatch, guard, call
+  | (state, _) => (state, Statement.skip)
 
 partial def eval (s : Statement) (state : State := default) : State :=
-  match step (state, s) with
-    | (state', Statement.skip) => state'
-    | (state', s') => eval s' state'
+  match evalStep (state, s) with
+  | (state', Statement.skip) => state'
+  | (state', s') => eval s' state'
 
 def test := [simpl|
   X :== 10;
